scratch/dp/DP_Lifting.thy
@@ -1,10 +1,10 @@
 theory DP_Lifting
-  imports Main "./Monad"
+  imports Main "./Monad" "HOL-Library.RBT_Mapping"
 begin
 
   (* Types *)
 type_synonym ('a,'M,'b) fun_lifted = "'a \<Rightarrow> ('M,'b) state" ("_ ==_\<Longrightarrow> _" [3,1000,2] 2)
-type_synonym ('a,'b) dpfun = "'a ==('a\<rightharpoonup>'b)\<Longrightarrow> 'b" (infixr "\<Rightarrow>\<^sub>T" 2)
+type_synonym ('a,'b) dpfun = "'a ==('a, 'b) mapping\<Longrightarrow> 'b" (infixr "\<Rightarrow>\<^sub>T" 2)
 term 0 (**)
   
   (* Basics *)
@@ -17,7 +17,7 @@ translations
   "\<lambda>\<^sub>T v. e" \<rightharpoonup> "\<langle>\<lambda> v. e\<rangle>"
 
 definition fun_app_lifted :: "('M,'a =='M\<Longrightarrow> 'b) state \<Rightarrow> ('M,'a) state \<Rightarrow> ('M,'b) state" (infixl "." 999) where
-  "f\<^sub>T . x\<^sub>T \<equiv> exec { f \<leftarrow> f\<^sub>T; x \<leftarrow> x\<^sub>T; f x }"
+  "f\<^sub>T . x\<^sub>T \<equiv> do { f \<leftarrow> f\<^sub>T; x \<leftarrow> x\<^sub>T; f x }"
 term 0 (**)
   
 lemma fun_app_lifted_elim1:
@@ -41,20 +41,20 @@ lemma return_app_return:
   unfolding fun_app_lifted_def left_identity ..
 term 0 (**)
   
-definition checkmem :: "'param \<Rightarrow> ('param \<rightharpoonup> 'result, 'result) state \<Rightarrow> ('param \<rightharpoonup> 'result, 'result) state" where
-  "checkmem param calc \<equiv> exec {
+definition checkmem :: "'param \<Rightarrow> (('param, 'result) mapping, 'result) state \<Rightarrow> (('param, 'result) mapping, 'result) state" where
+  "checkmem param calc \<equiv> do {
     M \<leftarrow> get;
-    case M param of
+    case Mapping.lookup M param of
       Some x \<Rightarrow> return x
-    | None \<Rightarrow> exec {
+    | None \<Rightarrow> do {
         x \<leftarrow> calc;
         M' \<leftarrow> get;
-        put (M'(param\<mapsto>x));
+        put (Mapping.update param x M');
         return x
       }
   }"
   
-abbreviation checkmem_eq :: "('param \<Rightarrow>\<^sub>T 'result) \<Rightarrow> 'param \<Rightarrow> ('param \<rightharpoonup> 'result, 'result) state \<Rightarrow> bool" ("_$ _ =CHECKMEM= _" [1000,51] 51) where
+abbreviation checkmem_eq :: "('param \<Rightarrow>\<^sub>T 'result) \<Rightarrow> 'param \<Rightarrow> (('param, 'result) mapping, 'result) state \<Rightarrow> bool" ("_$ _ =CHECKMEM= _" [1000,51] 51) where
   "(dp\<^sub>T$ param =CHECKMEM= calc) \<equiv> (dp\<^sub>T param = checkmem param calc)"
 term 0 (**)
   
@@ -112,7 +112,7 @@ lemma
 definition map\<^sub>T :: "('M, ('a =='M\<Longrightarrow> 'b) =='M\<Longrightarrow> 'a list =='M\<Longrightarrow> 'b list) state" where
   "map\<^sub>T \<equiv> lift_3 map\<^sub>T'"
 
-lemma map\<^sub>T_map\<^sub>T': "map\<^sub>T . f\<^sub>T . xs\<^sub>T = exec {f \<leftarrow> f\<^sub>T; xs \<leftarrow> xs\<^sub>T; map\<^sub>T' f xs}"
+lemma map\<^sub>T_map\<^sub>T': "map\<^sub>T . f\<^sub>T . xs\<^sub>T = do {f \<leftarrow> f\<^sub>T; xs \<leftarrow> xs\<^sub>T; map\<^sub>T' f xs}"
   unfolding map\<^sub>T_def lift_3_def fun_app_lifted_def left_identity bind_assoc ..
 term 0 (**)
   
