scratch/Scratch_Wfrec.thy
@@ -1,0 +1,51 @@
+theory Scratch_Wfrec
+  imports Main "HOL-Library.Old_Recdef" "dp/DP_CrelVS" Rewrite
+begin
+
+consts fib :: "nat \<Rightarrow> int"
+recdef fib "measure id"
+  "fib 0 = 1"
+  "fib (Suc 0) = 1"
+  "fib (Suc (Suc n)) = plus (fib (Suc n)) (fib n)"
+print_theorems
+
+consts fibT :: "nat \<Rightarrow>\<^sub>T int"
+recdef fibT "measure id"
+  "fibT$ 0 =CHECKMEM= \<langle>1\<rangle>"
+  "fibT$ (Suc 0) =CHECKMEM= \<langle>1\<rangle>"
+  "fibT$ (Suc (Suc n)) =CHECKMEM= plus\<^sub>T . (fibT (Suc n)) . (fibT n)"
+
+print_theorems
+thm wfrec_fixpoint
+
+context dp_consistency
+begin
+context includes lifting_syntax
+begin
+lemma
+  assumes "wf wfR"
+  assumes "adm_wf wfR body"
+  assumes "adm_wf wfR bodyT"
+  assumes "((op = ===>\<^sub>T op =) ===> (op = ===>\<^sub>T op =)) (body) (bodyT)"
+  shows "(op = ===>\<^sub>T op =) (wfrec wfR body) (wfrec wfR bodyT)"
+proof -
+  show ?thesis
+    apply (rule rel_funI)
+    apply clarsimp
+    subgoal for x
+      using assms(1) apply (induction x rule: wf_induct_rule)
+      subgoal premises IH for x 
+        thm IH
+        apply (rewrite in "_ body" wfrec_fixpoint)
+        subgoal using assms(1) .
+        subgoal using assms(2) .
+        apply (rewrite in "_ bodyT" wfrec_fixpoint)
+        subgoal using assms(1) .
+        subgoal using assms(3) .
+        using IH assms(4)[THEN rel_funD, OF rel_funI, THEN rel_funD
+            , where x1="wfrec wfR body" and y1="wfrec wfR bodyT" and x=x and y=x
+            , simplified
+            ]
+        ML_val \<open>@{method rewrite}\<close>
+end
+end
