scratch/dp/example/Bellman_Ford.thy
@@ -1,0 +1,39 @@
+theory Bellman_Ford
+  imports "../DP_Lifting" "../DP_CRelVS" "../DP_Proof"
+begin                                        
+  
+consts n :: nat
+consts W :: "nat \<Rightarrow> nat \<Rightarrow> int"
+term 0 (**)
+  
+  (*
+fun bf :: "nat\<times>nat \<Rightarrow> int" where
+  "bf (0,j) = W 0 j"
+| "bf (Suc k, j) = fold min [bf (k, i) + W i j. i \<leftarrow> [0..<n]] (bf (k, j))"
+term 0 (**)
+*)
+  
+fun bf :: "nat\<times>nat \<Rightarrow> int" where
+  "bf (0, j) = W 0 j"
+| "bf (Suc k, j) =
+    fold
+      (min)
+      (map
+          (\<lambda>i. plus (W i j) (bf (k, i)))
+          (upt 0 n))
+      (bf (k, j))"
+thm bf.simps
+thm bf.induct
+term 0 (**)
+
+ML_file \<open>../scratch/Transform.ML\<close>
+local_setup \<open>
+lift_fun NONE
+\<close>
+print_theorems
+
+interpretation bf: dp_consistency bf .
+
+lemma "bf.consistentDP bf\<^sub>T"
+  by (dp_match induct: bf\<^sub>T.crel_vs_induct simp: bf.simps simp\<^sub>T: bf\<^sub>T.simps)
+end
