scratch/dp/example/Fibonacci.thy
@@ -1,0 +1,89 @@
+theory Fibonacci
+  imports "../DP_Lifting" "../DP_CRelVS" "../DP_Proof"
+begin
+  
+  (*
+fun fib :: "nat \<Rightarrow> int option" where
+  "fib 0 = Some 0"
+| "fib (Suc 0) = Some 1"
+| "fib (Suc (Suc n)) = (case (fib (Suc n), fib n) of (Some f1, Some f0) \<Rightarrow> Some (f1 + f0) | _ \<Rightarrow> None)"
+term 0 (**)
+*)
+
+fun fib :: "nat \<Rightarrow> int option" where
+  "fib 0 = Some 0"
+| "fib (Suc 0) = Some 1"
+| "fib (Suc (Suc n)) = case_prod
+      (\<lambda>of1 of0. case_option
+        None
+        (\<lambda>f1. case_option
+          None
+          (\<lambda>f0. Some (f1 + f0))
+          of0)
+        of1)
+      (Pair (fib (Suc n)) (fib n))"
+
+ML_file \<open>../Transform.ML\<close>
+local_setup \<open>
+lift_fun NONE;
+\<close>
+
+interpretation fib: dp_consistency fib .
+
+lemma fib\<^sub>T_correct:
+  "fib.consistentDP fib\<^sub>T"
+  by (dp_match induct: fib\<^sub>T.induct simp: fib.simps simp\<^sub>T: fib\<^sub>T.simps)
+
+definition fib\<^sub>T_entry :: "nat \<Rightarrow> int option" where
+  "fib\<^sub>T_entry n \<equiv> fst (runState (fib\<^sub>T n) Mapping.empty)"
+
+lemma fib\<^sub>T_entry_correct:
+  "fib\<^sub>T_entry = fib"
+  unfolding fib\<^sub>T_entry_def using fib.consistentDP_entry[OF fib\<^sub>T_correct] ..
+
+lemma option_case_distrib2:
+  "(case_option f1 f2 x) v = case_option (f1 v) (\<lambda>y. f2 y v) x"
+  by (auto split: option.split)
+  
+lemma prod_absorb:
+  "(case (case a of (c, d) \<Rightarrow> (f c d, g c d)) of
+  (p, q) \<Rightarrow> h p q) = (case a of (c, d) \<Rightarrow>
+  (h (f c d) (g c d)))"
+  by (auto split: prod.splits)
+
+thm case_prod_beta
+lemma Let_absorb:
+  "(let (a, b) = (let (c, d) = x in (p c d, q c d)) in f a b)
+ = (let (c, d) = x in f (p c d) (q c d))"
+  by (auto simp: Let_def split: prod.splits)
+
+schematic_goal "?x = runState (fib\<^sub>T (Suc (Suc n))) Mapping.empty"
+  unfolding fib\<^sub>T.simps
+  unfolding case_prod\<^sub>T_def
+  unfolding checkmem_def
+  unfolding unlift_33_def
+  unfolding fun_app_lifted_def
+  unfolding return_def
+  unfolding bind_def
+  unfolding option.case_distrib option_case_distrib2
+  unfolding state.sel
+  unfolding Let_absorb
+  unfolding Let_def
+  unfolding state.sel
+  unfolding prod.case
+  unfolding state.sel
+  unfolding prod.case
+  unfolding prod_absorb
+  unfolding state.sel state.collapse
+  unfolding prod.case_distrib option.case_distrib
+  unfolding get_def put_def
+  unfolding state.sel
+  unfolding prod.case
+  unfolding prod_absorb
+  unfolding option_case_distrib2
+  unfolding prod_absorb
+  oops
+
+term 0 (*
+export_code fib\<^sub>T_entry in SML
+end
