scratch/dp/example/Grid_Path.thy
@@ -1,0 +1,96 @@
+theory Grid_Path
+  imports "../DP_CRelVS" "../DP_Lifting" "../DP_Proof"
+begin
+(*
+definition lift_option_choice :: "('a \<Rightarrow> 'a \<Rightarrow> 'a) \<Rightarrow> 'a option \<Rightarrow> 'a option \<Rightarrow> 'a option" where
+  "lift_option_choice \<equiv> \<lambda>f v0 v1.
+    case v0 of
+      None \<Rightarrow> (case v1 of
+        None \<Rightarrow> None
+      | Some y \<Rightarrow> Some y)
+    | Some x \<Rightarrow> (case v1 of
+      None \<Rightarrow> Some x
+      | Some y \<Rightarrow> Some (f x y))"
+
+definition lift_option_choice :: "('a \<Rightarrow> 'a \<Rightarrow> 'a) \<Rightarrow> 'a option \<Rightarrow> 'a option \<Rightarrow> 'a option" where
+  "lift_option_choice \<equiv> \<lambda>f. \<lambda>v0. \<lambda>v1.
+    case_option
+      (case_option
+        None
+        (\<lambda>y. Some y)
+        v1)
+      (\<lambda>x. (case_option
+        (Some x)
+        (\<lambda>y. Some (f x y))
+        v1))
+      v0"
+
+abbreviation min_opt :: "'a::ord option \<Rightarrow> 'a option \<Rightarrow> 'a option" where
+  "min_opt \<equiv> lift_option_choice min"
+term 0 (**)
+
+definition lift_option_choice\<^sub>T :: "('M, ('a =='M\<Longrightarrow> 'a =='M\<Longrightarrow> 'a) =='M\<Longrightarrow> 'a option =='M\<Longrightarrow> 'a option =='M\<Longrightarrow> 'a option) state" where
+  "lift_option_choice\<^sub>T \<equiv> \<lambda>\<^sub>Tf v0 v1.
+    case_option\<^sub>T
+    . (case_option\<^sub>T
+      . \<langle>None\<rangle>
+      . (\<lambda>\<^sub>T y. Some\<^sub>T . \<langle>y\<rangle>)
+      . \<langle>v1\<rangle>)
+    . (\<lambda>\<^sub>T x. case_option\<^sub>T
+      . (Some\<^sub>T . \<langle>x\<rangle>)
+      . (\<lambda>\<^sub>T y. Some\<^sub>T . (\<langle>f\<rangle> . \<langle>x\<rangle> . \<langle>y\<rangle>))
+      . \<langle>v1\<rangle>)
+    . \<langle>v0\<rangle>"
+  
+abbreviation min_opt\<^sub>T :: "('M, 'a::ord option =='M\<Longrightarrow> 'a option =='M\<Longrightarrow> 'a option) state" where
+  "min_opt\<^sub>T \<equiv> lift_option_choice\<^sub>T . min\<^sub>T"
+
+context dp_consistency begin
+lemma [transfer_rule]: "crel_vs ((R ===>\<^sub>T R ===>\<^sub>T R) ===>\<^sub>T rel_option R ===>\<^sub>T rel_option R ===>\<^sub>T rel_option R) lift_option_choice lift_option_choice\<^sub>T"
+  unfolding lift_option_choice_def lift_option_choice\<^sub>T_def by transfer_prover
+end
+*)
+
+definition "min_opt a b \<equiv>
+  case (a, b) of
+    (None, None) \<Rightarrow> None
+  | (Some a0, None) \<Rightarrow> Some a0
+  | (None, Some b0) \<Rightarrow> Some b0
+  | (Some a0, Some b0) \<Rightarrow> Some (min a0 b0)"
+term 0 (**)
+
+context
+  fixes W :: "nat \<Rightarrow> nat \<Rightarrow> nat option"
+begin
+
+fun ed :: "nat\<times>nat \<Rightarrow> nat option" where
+  "ed (0, 0) = W 0 0"
+| "ed (0, Suc j) = case_option None (\<lambda>prev.
+                     case_option None (\<lambda>here.
+                       Some (plus prev here)
+                     ) (W 0 (Suc j))
+                   ) (ed (0, j))"
+| "ed (Suc i, 0) = case_option None (\<lambda>prev.
+                     case_option None (\<lambda>here.
+                       Some (plus prev here)
+                     ) (W (Suc i) 0)
+                   ) (ed (i, 0))"
+| "ed (Suc i, Suc j) = case_option None (\<lambda>prev.
+                         case_option None (\<lambda>here.
+                           Some (plus prev here)
+                         ) (W (Suc i) (Suc j))
+                       ) (min_opt (ed (i, j)) (min_opt (ed (Suc i, j)) (ed (i, Suc j))))"
+
+ML_file \<open>../scratch/Transform.ML\<close>
+local_setup \<open>
+lift_fun NONE;
+\<close>
+print_theorems
+
+interpretation ed: dp_consistency ed .
+
+term 0 (**)
+lemma "ed.consistentDP ed\<^sub>T"
+  by (dp_match induct: ed\<^sub>T.induct simp: ed.simps simp\<^sub>T: ed\<^sub>T.simps)
+
+end
