scratch/dp/example/Knapsack.thy
@@ -1,0 +1,25 @@
+theory Knapsack
+  imports "../DP_CRelVS" "../DP_Proof"
+begin
+context (* Knapsack *)
+  fixes w :: "nat \<Rightarrow> nat"
+begin
+  
+fun su :: "nat\<times>nat \<Rightarrow> nat" where
+  "su (0, W) = (if W < w 0 then 0 else w 0)" |
+  "su (Suc i, W) = (if W < w (Suc i)
+    then su (i, W)
+    else max (su (i, W)) (w i + su (i, W - w i)))"
+ML_file \<open>../scratch/Transform.ML\<close>
+local_setup \<open>
+lift_fun NONE;
+\<close>
+print_theorems
+
+interpretation su: dp_consistency su .
+
+lemma "su.consistentDP su\<^sub>T"
+  by (dp_match induct: su\<^sub>T.induct simp: su.simps simp\<^sub>T: su\<^sub>T.simps)
+
+end
+end
