scratch/dp/example/Longest_Path.thy
@@ -1,0 +1,32 @@
+theory Longest_Path
+  imports "../DP_Lifting" "../DP_CRelVS" "../DP_Proof"
+begin
+
+context (* Longest path *)
+  fixes v :: "nat \<Rightarrow> nat"
+    and p :: "nat \<Rightarrow> nat"
+  assumes p_lt: "p (Suc j) < Suc j"
+begin
+
+
+text \<open>Dimensionality given by i\<close>
+function wis :: "nat \<Rightarrow> nat" where
+  "wis 0 = 0" |
+  "wis (Suc i) = max (wis (p (Suc i)) + v i) (wis i)"
+  by pat_completeness auto
+termination
+  by (relation "(\<lambda>p. size p) <*mlex*> {}") (auto intro: wf_mlex mlex_less simp: p_lt)
+
+ML_file \<open>../scratch/Transform.ML\<close>
+local_setup \<open>
+lift_fun NONE;
+\<close>
+print_theorems
+
+interpretation wis: dp_consistency wis .
+
+lemma "wis.consistentDP wis\<^sub>T"
+  by (dp_match induct: wis.induct simp: wis.simps simp\<^sub>T: wis\<^sub>T.simps)
+end
+
+end
